refactored to any wf type

src/FairBeh.v
@@ -6,8 +6,6 @@ Export ITreeNotations.
 
 Require Import Coq.Classes.RelationClasses.
 
-Require Import Lia.
-
 Set Implicit Arguments.
 
 Section OBS.
@@ -78,83 +76,89 @@ Module Flag.
 
 End Flag.
 
-Section INDEX.
-  Lemma nat_ind
-        (P: nat -> Prop)
-        (ZERO: P O)
-        (SUCC: forall a (IND: P a), P (S a))
-    :
-    forall n, P n.
-  Proof.
-    revert_until P. revert P. fix IH 4. i. destruct n; auto.
-    eapply SUCC. eapply IH. auto. i. eapply SUCC. auto.
-  Qed.
+(* Section INDEX. *)
+(*   Lemma nat_ind *)
+(*         (P: nat -> Prop) *)
+(*         (ZERO: P O) *)
+(*         (SUCC: forall a (IND: P a), P (S a)) *)
+(*     : *)
+(*     forall n, P n. *)
+(*   Proof. *)
+(*     revert_until P. revert P. fix IH 4. i. destruct n; auto. *)
+(*     eapply SUCC. eapply IH. auto. i. eapply SUCC. auto. *)
+(*   Qed. *)
 
-  Lemma nat_strong_ind
-        (P: nat -> Prop)
-        (ZERO: P O)
-        (SUCC: forall a (STR: forall b (LT: lt b (S a)), P b), P (S a))
-    :
-    forall n, P n.
-  Proof.
-    cut (forall a b (LT: lt b (S a)), P b).
-    { i. eapply H. instantiate (1:=n). auto. }
-    induction a; i; auto.
-    { inv LT; auto. inv H0. }
-    unfold lt in LT. inv LT.
-    { eapply SUCC. auto. }
-    eapply IHa. lia.
-  Qed.
+(*   Lemma nat_strong_ind *)
+(*         (P: nat -> Prop) *)
+(*         (ZERO: P O) *)
+(*         (SUCC: forall a (STR: forall b (LT: lt b (S a)), P b), P (S a)) *)
+(*     : *)
+(*     forall n, P n. *)
+(*   Proof. *)
+(*     cut (forall a b (LT: lt b (S a)), P b). *)
+(*     { i. eapply H. instantiate (1:=n). auto. } *)
+(*     induction a; i; auto. *)
+(*     { inv LT; auto. inv H0. } *)
+(*     unfold lt in LT. inv LT. *)
+(*     { eapply SUCC. auto. } *)
+(*     eapply IHa. lia. *)
+(*   Qed. *)
 
-  Lemma aux2: well_founded lt.
-  Proof.
-    ii. induction a using nat_strong_ind.
-    { econs. i. inv H. }
-    econs. i. eapply STR. auto.
-  Qed.
+(*   Lemma aux2: well_founded lt. *)
+(*   Proof. *)
+(*     ii. induction a using nat_strong_ind. *)
+(*     { econs. i. inv H. } *)
+(*     econs. i. eapply STR. auto. *)
+(*   Qed. *)
 
-End INDEX.
+(* End INDEX. *)
 
 
 Class ID : Type := mk_id { id: Type }.
-Class WFO : Type :=
-  mk_wfo {
-      ord: Type;
-      lt: (ord -> ord -> Prop);
-      wf: well_founded lt;
-      le: (ord -> ord -> Prop) := fun o1 o2 => (eq o1 o2) \/ (lt o1 o2);
-    }.
 
-Lemma wfo_strong_ind
-      (wfo: WFO) (P: ord -> Prop)
-      (ZERO: P O)
-      (SUCC: forall a (STR: forall b (LT: lt b (S a)), P b), P (S a))
-  :
-  forall n, P n.
-Proof.
-  cut (forall a b (LT: lt b (S a)), P b).
-  { i. eapply H. instantiate (1:=n). auto. }
-  induction a; i; auto.
-  { inv LT; auto. inv H0. }
-  unfold lt in LT. inv LT.
-  { eapply SUCC. auto. }
-  eapply IHa. lia.
-Qed.
+Section WFTransitive.
+  Record WF: Type :=
+    mk_wf {
+        T: Type;
+        lt: (T -> T -> Prop);
+        wf: well_founded lt;
+        (* Tr: Transitive lt; *)
+        le: (T -> T -> Prop) := eq \2/ lt;
+      }.
 
-Global Program Instance WFO_lt_Transitive {wfo: WFO}: Transitive (@lt wfo).
-Next Obligation.
-  assert (WF: well_founded lt).
-  { destruct wfo. ss. }
-  depgen z. depgen x. induction (WF y); i.
-  eapply H0. 2,3: eauto.
+  (* Global Program Instance lt_Transitive {wf: WF} {TR: Transitive wf.(lt)}: Transitive wf.(lt). *)
+  (* Next Obligation. *)
+  (*   destruct wf0. ss. eapply TR; eauto. *)
+  (* Qed. *)
 
-Global Program Instance WFO_le_PreOrder {wfo: WFO}: PreOrder (@le wfo).
-Next Obligation.
-  ii. rr. left; auto.
-Qed.
-Next Obligation.
-  ii. unfold le in *. des; clarify; auto. unfold soft_update in *. specialize (H i). specialize (H0 i). lia.
-Qed.
+  Global Program Instance le_Reflexive {wf: WF}: Reflexive wf.(le).
+  Next Obligation.
+    unfold le. auto.
+  Qed.
+
+  Lemma WF_le_Trans
+        wf
+        (WFTR: Transitive wf.(lt))
+    :
+    Transitive wf.(le).
+  Proof.
+    unfold le. ii. destruct wf; ss. des; clarify; eauto.
+  Qed.
+
+  (* Global Program Instance le_PreOrder {wf: WF} {TR: Transitive wf.(lt)}: PreOrder wf.(le). *)
+  (* Next Obligation. *)
+  (*   unfold le. ii. destruct wf0; ss. des; clarify; eauto. *)
+  (* Qed. *)
+
+End WFTransitive.
+
+(* Class WF : Type := *)
+(*   mk_wf { *)
+(*       ord: Type; *)
+(*       lt: (ord -> ord -> Prop); *)
+(*       wf: well_founded lt; *)
+(*       le: (ord -> ord -> Prop) := fun o1 o2 => (eq o1 o2) \/ (lt o1 o2); *)
+(*     }. *)
 
 
 
@@ -162,9 +166,11 @@ Section EVENT.
 
   Context {Ident: ID}.
 
+  Definition fmap := id -> Flag.t.
+
   Variant eventE: Type -> Type :=
     | Choose (X: Type): eventE X
-    | Fair (m: id -> Flag.t): eventE unit
+    | Fair (m: fmap): eventE unit
     | Observe (fn: nat) (args: list nat): eventE nat
     | Undefined: eventE void
   .
@@ -176,26 +182,23 @@ End EVENT.
 Section STS.
 
   Context {Ident: ID}.
-  Context {WFOrder: WFO}.
+  Variable wf: WF.
 
   Definition state {R} := itree eventE R.
-  Definition imap := id -> ord.
+  Definition imap := id -> wf.(T).
 
   Definition soft_update (m0 m1: imap): Prop :=
-    forall i, le (m1 i) (m0 i).
+    forall i, wf.(le) (m1 i) (m0 i).
 
-  Global Program Instance soft_update_PreOrder: PreOrder soft_update.
+  Global Program Instance soft_update_Reflexive: Reflexive soft_update.
   Next Obligation.
-    ii. auto.
-  Qed.
-  Next Obligation.
-    ii. unfold soft_update in *. specialize (H i). specialize (H0 i). lia.
+    ii. reflexivity.
   Qed.
 
-  Definition fair_update (m0 m1: imap) (f: id -> Flag.t): Prop :=
+  Definition fair_update (m0 m1: imap) (f: fmap): Prop :=
     forall i, match f i with
-         | Flag.fail => Peano.lt (m1 i) (m0 i)
-         | Flag.emp => le (m1 i) (m0 i)
+         | Flag.fail => wf.(lt) (m1 i) (m0 i)
+         | Flag.emp => wf.(le) (m1 i) (m0 i)
          | Flag.success => True
          end.
 
@@ -209,12 +212,13 @@ Definition improves {R} (src tgt: @t R): Prop := tgt <1= src.
 Section BEHAVES.
 
   Context {Ident: ID}.
+  Variable wf: WF.
 
   Variant _diverge_index
-          (diverge_index: forall (R: Type) (idx: imap) (itr: @state _ R), Prop)
+          (diverge_index: forall (R: Type) (idx: imap wf) (itr: @state _ R), Prop)
           (R: Type)
     :
-    forall (idx: imap) (itr: @state _ R), Prop :=
+    forall (idx: imap wf) (itr: @state _ R), Prop :=
     | diverge_index_tau
         itr idx0
         (DIV: diverge_index _ idx0 itr)
@@ -246,7 +250,7 @@ Section BEHAVES.
     - econs 4; eauto.
   Qed.
 
-  Definition diverge_index: forall (R: Type) (idx: imap) (itr: state), Prop := paco3 _diverge_index bot3.
+  Definition diverge_index: forall (R: Type) (idx: imap wf) (itr: state), Prop := paco3 _diverge_index bot3.
 
   Hint Constructors _diverge_index.
   Hint Unfold diverge_index.
@@ -259,10 +263,10 @@ Section BEHAVES.
 
 
   Inductive _of_state
-            (of_state: forall (R: Type), imap -> (@state _ R) -> (@Tr.t R) -> Prop)
+            (of_state: forall (R: Type), (imap wf) -> (@state _ R) -> (@Tr.t R) -> Prop)
             (R: Type)
     :
-    imap -> (@state _ R) -> Tr.t -> Prop :=
+    (imap wf) -> (@state _ R) -> Tr.t -> Prop :=
   | done
       imap0 retv
     :
@@ -305,10 +309,10 @@ Section BEHAVES.
     _of_state of_state imap0 (Vis Undefined ktr) tr
   .
 
-  Definition of_state: forall (R: Type),  imap -> state -> Tr.t -> Prop := paco4 _of_state bot4.
+  Definition of_state: forall (R: Type),  (imap wf) -> state -> Tr.t -> Prop := paco4 _of_state bot4.
 
   Theorem of_state_ind:
-    forall (r: forall (R: Type), imap -> state -> Tr.t -> Prop) R (P: imap -> state -> Tr.t -> Prop),
+    forall (r: forall (R: Type), (imap wf) -> state -> Tr.t -> Prop) R (P: (imap wf) -> state -> Tr.t -> Prop),
       (forall imap0 retv, P imap0 (Ret retv) (Tr.done retv)) ->
       (forall imap0 st0, diverge_index imap0 st0 -> P imap0 st0 Tr.spin) ->
       (forall imap0 st0, P imap0 st0 Tr.nb) ->
@@ -364,11 +368,13 @@ Section BEHAVES.
   (*********************** upto ***********************)
   (****************************************************)
 
+  Hypothesis WFTR: Transitive wf.(lt).
+
   Variant diverge_imap_le_ctx
-          (diverge_index: forall R, imap -> (@state _ R) -> Prop)
+          (diverge_index: forall R, (imap wf) -> (@state _ R) -> Prop)
           R
     :
-    imap -> (@state _ R) -> Prop :=
+    (imap wf) -> (@state _ R) -> Prop :=
     | diverge_imap_le_ctx_intro
         imap0 imap1 st
         (DIV: @diverge_index R imap1 st)
@@ -388,8 +394,10 @@ Section BEHAVES.
     { econs 1. eapply rclo3_clo_base. econs 1; eauto. }
     { econs 2. eapply rclo3_clo_base. econs 1; eauto. }
     { econs 3. eapply rclo3_clo_base. econs 1. eauto. reflexivity.
-      clear - IMAP FAIR. unfold fair_update, soft_update in *. i. specialize (IMAP i). specialize (FAIR i).
-      des_ifs; nia.
+      clear - WFTR IMAP FAIR. unfold fair_update, soft_update in *. i. specialize (IMAP i). specialize (FAIR i).
+      des_ifs.
+      - unfold le in IMAP. des. rewrite IMAP in FAIR. auto. eapply WFTR; eauto.
+      - eapply WF_le_Trans; eauto.
     }
   Qed.
 
@@ -399,10 +407,10 @@ Section BEHAVES.
 
 
   Variant imap_le_ctx
-          (of_state: forall R, imap -> (@state _ R) -> (@Tr.t R) -> Prop)
+          (of_state: forall R, (imap wf) -> (@state _ R) -> (@Tr.t R) -> Prop)
           R
     :
-    imap -> (@state _ R) -> (@Tr.t R) -> Prop :=
+    (imap wf) -> (@state _ R) -> (@Tr.t R) -> Prop :=
     | imap_le_ctx_intro
         imap0 imap1 st tr
         (BEH: @of_state R imap1 st tr)
@@ -423,8 +431,10 @@ Section BEHAVES.
       eapply diverge_index_mon; eauto. i. gfinal. pclearbot. auto.
     }
     { econs. eapply rclo4_clo_base. econs; eauto. }
-    { econs. eapply IHBEH. reflexivity. clear - IMAP FMAP. unfold fair_update, soft_update in *.
-      i. specialize (FMAP i). specialize (IMAP i). des_ifs; lia.
+    { econs. eapply IHBEH. reflexivity. clear - WFTR IMAP FMAP. unfold fair_update, soft_update in *.
+      i. specialize (FMAP i). specialize (IMAP i). des_ifs.
+      - unfold le in IMAP. des. rewrite <- IMAP. auto. eapply WFTR; eauto.
+      - eapply WF_le_Trans; eauto.
     }
   Qed.
 
@@ -434,10 +444,10 @@ Section BEHAVES.
 
 
   Variant of_state_indC
-          (of_state: forall R, imap -> (@state _ R) -> (@Tr.t R) -> Prop)
+          (of_state: forall R, (imap wf) -> (@state _ R) -> (@Tr.t R) -> Prop)
           R
     :
-    imap -> (@state _ R) -> (@Tr.t R) -> Prop :=
+    (imap wf) -> (@state _ R) -> (@Tr.t R) -> Prop :=
   | of_state_indC_done
       imap0 retv
     :
@@ -608,9 +618,10 @@ End Beh.
 Section AUX.
 
   Context {Ident: ID}.
+  Variable wf: WF.
 
   Theorem of_state_ind2:
-    forall R (P: imap -> state -> Tr.t -> Prop),
+    forall R (P: (imap wf) -> state -> Tr.t -> Prop),
       (forall imap0 retv, P imap0 (Ret retv) (Tr.done retv)) ->
       (forall imap0 st0, Beh.diverge_index imap0 st0 -> P imap0 st0 Tr.spin) ->
       (forall imap0 st0, P imap0 st0 Tr.nb) ->
@@ -635,7 +646,7 @@ Section AUX.
         ,
           P imap0 (Vis (Fair fmap) ktr) tr) ->
       (forall imap0 ktr tr, P imap0 (Vis Undefined ktr) tr) ->
-      forall i s t, (@Beh.of_state _ R i s t) -> P i s t.
+      forall i s t, (@Beh.of_state _ _ R i s t) -> P i s t.
   Proof.
     i. eapply Beh.of_state_ind; eauto.
     { i. eapply H3; eauto. pfold. eapply Beh.of_state_mon; eauto. }
