src/Adequacy.v
@@ -17,6 +17,7 @@ Set Implicit Arguments.
 Section ADEQ.
 
   Context {Ident: ID}.
+  Variable wf: WF.
 
   Lemma adequacy_spin
         R0 R1 (RR: R0 -> R1 -> Prop)
@@ -24,7 +25,7 @@ Section ADEQ.
         (SIM: sim RR psrc0 msrc0 ptgt0 mtgt0 ssrc0 stgt0)
         (SPIN: Beh.diverge_index mtgt0 stgt0)
     :
-    <<SPIN: Beh.diverge_index msrc0 ssrc0>>.
+    <<SPIN: Beh.diverge_index (wf:=wf) msrc0 ssrc0>>.
   Proof.
     ginit. revert_until RR. gcofix CIH. i. revert SPIN.
     induction SIM using @sim_ind2; i; clarify.
@@ -71,7 +72,7 @@ Section ADEQ.
           psrc0 ptgt0 msrc0 mtgt0 ssrc0 stgt0
           (SIM: sim (@eq R) psrc0 msrc0 ptgt0 mtgt0 ssrc0 stgt0)
     :
-    <<IMPR: Beh.improves (Beh.of_state msrc0 ssrc0) (Beh.of_state mtgt0 stgt0)>>.
+    <<IMPR: Beh.improves (Beh.of_state msrc0 ssrc0) (Beh.of_state (wf:=wf) mtgt0 stgt0)>>.
   Proof.
     ginit. revert_until R. gcofix CIH.
     i. rename x4 into tr. revert psrc0 ptgt0 msrc0 ssrc0 SIM.
